Evaluation.v
@@ -1,0 +1,732 @@
+Require Import Coq.Classes.EquivDec.
+Require Import Coq.Program.Equality.
+Require Import Coq.Program.Utils.
+Require Import Coq.Logic.Classical.
+Require Import List.
+Require Import Nat.
+Require Import Bool.Bool.
+Require Import Coq.Logic.Eqdep_dec.
+
+Require Graph.
+Require Import Util.
+
+Module Evaluation.
+
+  Export Graph.Graph.
+
+  Parameter Val : Type.
+  Definition Tag := list nat.
+
+  Definition State := Var -> Val.
+
+  Variable Val_dec : EqDec Val eq.
+  Variable Tag_dec : EqDec Tag eq.
+  Variable State_dec : EqDec State eq.
+
+  
+  Parameter start_tag : Tag.
+
+  Definition States := State -> Prop.
+  Definition Coord := prod Lab Tag.
+  Definition Conf := prod Coord State.
+
+  Hint Unfold Conf Coord.
+
+  Definition lab_of (k : Conf) :=
+    match k with
+      ((p, i), s) => p
+    end.
+
+    Parameter eff' : Lab * State -> option (Lab * State).
+  
+  Fixpoint eff_tag (k : Conf) : Tag
+    := match k with
+         (p, i, s)
+         => match eff' (p,s) with
+             Some (q , r)
+             => if is_back_edge p q
+               then match i with
+                    | nil => nil
+                    | n :: l => (S n) :: l
+                    end
+               else 
+                    let l' := @iter Tag (@tl nat) i (loop_exit p) in
+                    @iter Tag (@cons nat O) l' (loop_head q)
+                |
+             None => nil
+           end
+       end.
+
+  Definition eff (k : Conf) : option Conf
+    := match k with
+       | (p, i, s) => match eff' (p,s) with
+                  | None => None
+                  | Some (q, r) => Some (q, eff_tag k, r)
+                  end
+       end.
+
+    Lemma Conf_dec :
+    forall (x y : Conf), {x = y} + {x <> y}.
+  Proof.
+    intros.
+    destruct x as [[p i] s], y as [[q j] r].
+    destruct ((p, i, s) == (q, j, r)); firstorder.
+  Qed.
+  Instance conf_eq_eqdec : EqDec Conf eq := Conf_dec.
+
+
+  Definition start_coord := (root, start_tag) : Coord.
+
+  Definition is_effect_on (p q : Lab) :=
+    exists i i' s s', eff ((p, i), s) = Some ((q, i'), s').
+
+  Parameter edge_spec :
+    forall p q, is_effect_on p q -> p --> q.
+
+  Lemma step_conf_implies_edge :
+    forall p q i j s r, eff (p, i, s) = Some (q, j, r) -> (p --> q).
+  Proof.
+    intros.
+    eapply edge_spec. 
+    unfold is_effect_on. eauto.
+  Qed.
+
+  Parameter def_spec :
+    forall p q x, (exists i j s r, eff (p, i, s) = Some (q, j, r) /\ r x <> s x) ->
+                  is_def x p q = true.
+
+
+  (* TODO *)
+  Inductive Tr : Conf -> Type :=
+    | Init : forall s, Tr (root, start_tag, s)
+    | Step : forall k k', Tr k' -> eff k' = Some k -> Tr k.
+
+  Ltac inv_dep H Dec := inversion H; subst; 
+                        repeat match goal with
+                               | [ H0: @existT _ _ _ _ = @existT _ _ _ _  |- _ ] =>
+                                 apply inj_pair2_eq_dec in H0; try (apply Dec); subst
+                               end.
+
+  Ltac inv_tr H := inversion H; subst; 
+                   repeat match goal with
+                          | [ H0: @existT Conf _ _ _ = @existT _ _ _ _  |- _ ] => apply inj_pair2_eq_dec in H0; try (apply Conf_dec); subst
+                          end.
+
+  Definition Traces := forall k, Tr k -> Prop.
+  Definition Hyper := Traces -> Prop.
+
+  (* This is the concrete transformer for sets of traces *)
+  Definition sem_trace (ts : Traces) : Traces :=
+    fun k' => fun tr' => exists k tr step, ts k tr /\ tr' = (Step k' k tr step).
+
+  (* This is the hypertrace transformer.
+     Essentially, it lifts the trace set transformers to set of trace sets *)
+  Definition sem_hyper (T : Hyper) : Hyper :=
+    fun ts' => exists ts, T ts /\ ts' = sem_trace ts.
+
+   
+  Inductive In : forall k, Tr k -> Conf -> Prop :=
+    | In_At : forall k tr, In k tr k
+    | In_Other : forall l k k' tr' step, In k' tr' l -> In k (Step k k' tr' step) l.
+
+  Lemma tr_in_dec :
+    forall k' k t, {In k t k'} + {~ In k t k'}.
+  Proof.
+    intros k'.
+    induction t.
+    - destruct (conf_eq_eqdec (start_coord, s) k').
+      + left. rewrite <- e. econstructor.
+      + right. intro. apply c. inv_tr H. reflexivity.
+    - destruct (k == k').
+      + left. rewrite <- e0. constructor.
+      + inversion_clear IHt.
+        * left. econstructor. eassumption.
+        * right. intro. apply H. inv_tr H0; firstorder.
+  Qed.
+
+  Lemma in_succ_in k p q t :
+    In k t p -> p =/= k -> eff p = Some q -> In k t q.
+  Proof.
+    intros.
+    dependent induction t; inv_tr H; try firstorder.
+    destruct (p == k').
+    + rewrite e0 in *. clear e0.
+      inv_tr H; firstorder.
+      rewrite H1 in step1. injection step1; intros. symmetry in H3. subst. constructor.
+    + constructor. eauto.
+  Qed.
+
+  Lemma in_succ_exists p q i j s r t :
+    In (p, i, s) t (q, j, r) -> (exists k', eff (q, j, r) = Some k' /\ In (p, i, s) t k') \/ (p, i, s) = (q, j, r).
+  Proof.
+    intros Hin.
+    dependent induction t; inv_tr Hin; eauto.
+    destruct k' as [[a l] u].
+    left.
+    specialize (IHt a l u t).
+    destruct IHt; eauto.
+    + destruct H as [k' H]. exists k'. split; try constructor; firstorder.
+    + injection H; intros; subst. exists (p, i, s). firstorder. constructor.
+  Qed.
+
+  Lemma in_pred_exists p i s k t :
+    forall k' step, In k' (Step k' k t step) (p, i, s) ->
+    p =/= root ->
+    exists q j r, In k t (q, j, r) /\ eff (q, j, r) = Some (p, i, s).
+  Proof.
+    intros k' step Hin Hneq.
+    dependent induction t.
+    - inv_tr Hin.
+      + exists root, start_tag, s0. split; [ constructor | assumption ].
+      + inv_tr H3. firstorder.
+    - inv_tr Hin.
+      + destruct k as [[q j] r].
+        exists q, j, r. split; [ constructor | assumption ].
+      + edestruct IHt as [q [j [r [Hinq Hstep]]]]; try eassumption.
+        exists q, j, r. 
+        split; eauto using In.
+  Qed.
+
+
+  Parameter ivec_fresh : forall p i s k t, eff k = Some (p, i, s) ->
+                                      forall q j r, In k t (q, j, r) ->
+                                               j <> i.
+
+  Parameter ivec_det : forall q j r r' p i i' s s',
+      eff (q, j, r) = Some (p, i, s) ->
+      eff (q, j, r') = Some (p, i', s') ->
+      i = i'.
+
+  Inductive Precedes : forall k, Tr k -> Conf -> Conf -> Prop :=
+  | Pr_in : forall k t, Precedes k t k k
+  | Pr_cont : forall q q' p i j j' r' r s t step, Precedes (q', j', r') t (q, j, r) (q', j', r') -> 
+                                                  p =/= q ->
+                                                  Precedes (p, i, s) (Step (p, i, s) (q', j', r') t step) (q, j, r) (p, i, s)
+  | Pr_other : forall k' k t c c' step, Precedes k t c c' ->
+                                        Precedes k' (Step k' k t step) c c'.
+
+
+  Lemma precedes_implies_in_pred k t k' k'' :
+    Precedes k t k' k'' -> In k t k'.
+  Proof.
+    intros H.
+    dependent induction t.
+    - inv_tr H. constructor.
+    - inv_tr H; eauto using In.
+  Qed.
+
+  Lemma precedes_implies_in_succ k t k' k'' :
+    Precedes k t k' k'' -> In k t k''.
+  Proof.
+    intros H.
+    dependent induction t.
+    - inv_tr H. constructor.
+    - inv_tr H; eauto using In.
+  Qed.
+
+  Inductive Prefix : forall k, Tr k -> forall k', Tr k' -> Prop :=
+  | PrefixSame : forall k t, Prefix k t k t
+  | PrefixStep : forall k'' k' k step t t', Prefix k t k' t' ->
+                                       Prefix k t k'' (Step k'' k' t' step).
+    
+  Lemma precedes_prefix k t c c' : 
+    Precedes k t c c' ->
+    exists tr, Prefix c' tr k t /\ Precedes c' tr c c'.
+  Proof.
+    intros Hprec.
+    dependent induction t.
+    + inv_tr Hprec.
+      - eexists. split; eauto using Prefix.
+    + inv_tr Hprec.
+      - eexists. split; constructor.
+      - eexists. split; [ constructor | eassumption ].
+      - eapply IHt in H4.
+        destruct H4 as [tr [Hprefix Hprec']].
+        exists tr. split; eauto using Prefix. 
+  Qed.
+
+  Lemma precedes_prefix_inv k t c c' l tr k' step : 
+    Precedes k' (Step k' k t step) c c' ->
+    Prefix k t l tr ->
+    forall l' step', Precedes l' (Step l' l tr step') c c'.
+  Proof.
+    intros Hprec Hprefix.
+    dependent induction Hprefix; intros l' step'.
+    + cut (Some k' = Some l'); intros.
+      - inject H.
+        cut (step = step'); intros; subst; try eassumption.
+        clear Hprec. destruct step'. apply UIP_refl.
+      - rewrite <- step. eassumption.
+    + constructor. eapply IHHprefix. eassumption.
+  Qed.
+
+    Lemma in_prefix k t c : 
+    In k t c ->
+    exists pt, Prefix c pt k t /\
+          In c pt c.
+  Proof.
+    intros.
+    dependent induction t.
+    + inv_tr H. exists (Init s). split; constructor.
+    + inv_tr H.
+    - exists tr0. split; constructor.
+    - eapply IHt in H4. destruct H4 as [pt [Hprefix Hin]].
+      exists pt. split; [ constructor | ]; eassumption.
+  Qed.
+  
+  Lemma in_prefix_in k t c k' t' :
+    In k t c ->
+    Prefix k t k' t' ->
+    In k' t' c.
+  Proof.
+    intros Hin Hprefix. dependent induction Hprefix; eauto using In.
+  Qed.
+
+  Fixpoint last_inst_of (l : Lab) (k : Conf) (t : Tr k) : option Tag :=
+    match t with
+    | (Init s) => if l == root then Some start_tag else None
+    | (Step (q, j, _) k t _) => if (l == q) then Some j else last_inst_of l k t
+    end.
+
+  Lemma last_inst_precedes_inv_helper q j r q' j' r' t e br m w :
+    Precedes (q, j, r) (Step (q, j, r) (q', j', r') t e)
+            (br, m, w) (q, j, r) ->
+    br =/= q ->
+    Precedes (q', j', r') t (br, m, w) (q', j', r').
+  Proof.
+    intros Hprec Hneq.
+    inv_tr Hprec.
+    - contradiction Hneq; reflexivity.
+    - eauto.
+    - exfalso. eapply (ivec_fresh _ _ _ _ _ step0); [ |reflexivity].
+      eauto using precedes_implies_in_succ. 
+  Qed.
+
+  Lemma last_inst_precedes_inv q j r br m w t : 
+    Precedes (q, j, r) t (br, m, w) (q, j, r) ->
+    last_inst_of br (q, j, r) t = Some m.
+  Proof.
+    intros Hprec.
+    dependent induction t; intros; simpl.
+    + destruct (br == root).
+      rewrite e in *. clear e.
+      inv_tr Hprec.
+      - reflexivity.
+      - inv_tr Hprec.
+        contradiction c; reflexivity.
+    + destruct k' as [[q' j'] r']. 
+      destruct (br == q).
+      * rewrite e0 in *. clear e0.
+        inv_tr Hprec; try reflexivity.
+        - contradiction H10; reflexivity.
+        - exfalso. eapply ivec_fresh. eapply step0.
+          eapply precedes_implies_in_succ. eassumption. reflexivity.
+      * eapply IHt; try reflexivity. 
+        eauto using last_inst_precedes_inv_helper.
+  Qed.
+
+  Lemma last_inst_precedes q j r br m t : 
+    last_inst_of br (q, j, r) t = Some m -> 
+    exists w, Precedes (q, j, r) t (br, m, w) (q, j, r).
+  Proof.
+    intros Hin.
+    dependent induction t; intros; simpl in Hin.
+    + destruct (br == root).
+      - rewrite e in *. clear e.
+        injection Hin; intros; subst.
+        exists r. constructor.
+      - inversion Hin.
+    + destruct k' as [[q' j'] r']. 
+      destruct (br == q).
+      * rewrite e0 in *. clear e0.
+        injection Hin; intros; subst; clear Hin.
+        exists r. constructor.
+      * eapply IHt in Hin; eauto.
+        destruct Hin as [w Hprec].
+        exists w. symmetry in c. eauto using Precedes.
+  Qed.
+
+(*  Definition unique_preceding q p :=
+      forall k k' t t' j j' i r r' s s',
+      Precedes k t (q, j, r) (p, i, s) ->
+      Precedes k' t' (q, j', r') (p, i, s') ->
+      j' = j.*)
+
+
+  Definition step_exists_path {q p} {j i} {r s} (step : eff (q, j, r) = Some (p, i, s)) :=
+           (PathStep q q p (PathInit q) (step_conf_implies_edge q p j i r s step)).
+
+  Lemma path_for_trace k tr k' (Hin : In k tr k') :
+    { p: Path (lab_of k') (lab_of k) | forall q, PathIn q p -> exists j r, In k tr (q, j, r) }.
+  Proof.
+    destruct k as [[q j] r], k' as [[p i] s]. simpl.
+    dependent induction tr; intros.
+    + simpl.
+      enough (p = root).
+      - subst. exists (PathInit root). simpl. intros. rewrite H. eauto.
+      - inv_tr Hin; reflexivity.
+   + destruct k' as [[q' j'] r']; simpl in *.
+     destruct (p == q).
+     * rewrite e0. clear e0. exists (PathInit q). intros. 
+       inversion_clear H; subst. exists j, r. constructor.
+     * edestruct IHtr; eauto. inv_tr Hin.
+       - contradiction c; reflexivity.
+       - eapply H3.
+       - exists (PathStep p q' q x (step_conf_implies_edge q' q _ _ _ _ e)).
+         intros. simpl in H. inversion_clear H.
+         ++ rewrite H0. exists j, r. constructor.
+         ++ eapply e0 in H0. destruct H0 as [j0 [r0 H0]].
+            exists j0, r0. eauto using In.
+  Qed.
+
+  Lemma not_in_trace_exists_path (q : Lab) (k k' : Conf) (t : Tr k) (Hin : In k t k') : 
+    ~ (exists j r, In k t (q, j, r)) ->
+    ~ PathIn q (proj1_sig (path_for_trace k t k' Hin)).
+  Proof.
+    intros Hnin.
+    intro. apply Hnin. clear Hnin.
+    remember (path_for_trace k t k' Hin) as p.
+    clear Heqp.
+    destruct p as [p Hpin]; simpl in *.
+    eauto.
+  Qed.
+  
+  Lemma start_no_tgt :
+    forall i' s' k, eff k = Some (root, i', s') -> False.
+  Proof.
+    intros. 
+    destruct k as [[p i] s].
+    unfold start_coord in H.
+    cut (is_effect_on p root); intros.
+    apply edge_spec in H0.
+    eapply root_no_pred. eassumption.
+    unfold is_effect_on.
+    exists i, i', s, s'. 
+    assumption.
+  Qed.
+
+  Lemma precedes_self k t :
+    forall c, In k t c -> Precedes k t c c.
+  Proof.
+    intros c H.
+    destruct c as [[p i] s].
+    dependent induction t.
+    + inv_tr H. constructor.
+    + destruct k' as [[q j] r].
+      inv_tr H; eauto using Precedes.
+  Qed.
+
+  Lemma precedes_step_inv :
+    forall k k' t step p s, Precedes k' (Step k' k t step) p s ->
+                            lab_of p =/= lab_of s ->
+                            In k t p.
+  Proof.
+    intros.
+    inv_tr H.
+    - firstorder.
+    - eapply precedes_implies_in_pred. eauto.
+    - eapply precedes_implies_in_pred. eauto.
+  Qed.
+
+  Lemma precedes_incl k t c c' :
+    Precedes k t c c' -> exists t', Precedes c' t' c c'.
+  Proof.
+    intros. dependent induction t; inv_tr H; eauto.
+  Qed.
+
+  Lemma in_exists_pred p i s k t :
+    forall k' step, In k' (Step k' k t step) (p, i, s) ->
+    p <> root ->
+    exists q j r, In k t (q, j, r) /\ eff (q, j, r) = Some (p, i, s).
+  Proof.
+    intros k' step H Hneq.
+    dependent induction t; inv_tr H.
+    - exists root, start_tag, s0. split; [ constructor | eauto ].
+    - inv_tr H4. firstorder.
+    - destruct k as [[q j] r]. exists q, j, r.
+      split; [ constructor | eauto ].
+    - eapply IHt in H4; eauto. destruct H4 as [q [j [r [Hin Hstep]]]].
+      exists q, j, r. split; [ constructor |]; eauto.
+  Qed.
+
+  Lemma precedes_succ k t :
+    forall q j r q' j' r' p i s k' step, Precedes k t (q', j', r') (q, j, r) ->
+                                         eff (q, j, r) = Some (p, i, s) ->
+                                         p =/= q' ->
+                                         Precedes k' (Step k' k t step) (q', j', r') (p, i, s).
+  Proof.
+    dependent induction t.
+    - intros.
+      destruct k' as [[p' i'] s'].
+      inv_tr H. enough (Some (p, i, s0) = Some (p', i', s')).
+      injection H2; intros; subst. eauto using Precedes.
+      rewrite <- H0. eauto.
+    - intros. inv_tr H.
+      * injection H5; intros; subst.
+        enough (Some k'0 = Some (p, i, s)). injection H2; intros; subst.
+        eauto using Precedes.
+        rewrite <- step. eassumption.
+      * enough (Some k'0 = Some (p, i, s)). injection H4; intros; subst.
+        eauto using Precedes.
+        rewrite <- step. eassumption.
+      * eauto using Precedes.
+  Qed.
+
+  Lemma precedes_step k t q j r to i s :
+    forall k' step, In k t (q, j, r) ->
+                    to =/= q ->
+                    eff (q, j, r) = Some (to, i, s) ->
+                    Precedes k' (Step k' k t step) (q, j, r) (to, i, s).
+  Proof.
+    intros k' step Hin Hneq Hstep.
+    dependent induction t.
+    - inv_tr Hin.
+      enough (Some k' = Some (to, i, s0)).
+      injection H; intros; subst. eauto using Precedes.
+      rewrite <- step. eassumption.
+    - inv_tr Hin.
+      * enough (Some k'0 = Some (to, i, s)).
+        injection H; intros; subst. eauto using Precedes.
+        rewrite <- step. eassumption.
+      * eauto using Precedes.
+  Qed.
+    
+  Lemma no_def_untouched :
+    forall p q x, is_def x q p = false -> forall i j s r, eff (q, j, r) = Some (p, i, s) -> r x = s x.
+  Proof.
+    intros.
+    specialize (def_spec q p x).
+    cut (forall (a b : Prop), (a -> b) -> (~ b -> ~ a)); intros Hrev; [| eauto].
+    assert (Hds := def_spec).
+    eapply Hrev in Hds.
+    - cut (forall x y : Val, ~ (x <> y) -> x = y).
+      * intros.
+        apply H1; clear H1.
+        intro. apply Hds.
+        exists j; exists i; exists r; exists s; eauto.
+      * intros y z. destruct (equiv_dec y z); intros; auto.
+        exfalso. apply H1. auto.
+    - intro.
+      rewrite H in H1.
+      inversion H1.
+  Qed.
+
+    
+  Definition lab_tag_matches (l : Lab) (j : Tag) (k : Conf) : bool :=
+    match k with
+    | ((p, i), s) => (j ==b i) && (l ==b p) 
+    end.
+
+  Fixpoint label_tag_in_trace (l : Lab) (i : Tag) (k : Conf) (t : Tr k) : bool :=
+    match t with
+    | (Init s) => lab_tag_matches l i (root, start_tag, s)
+    | (Step k' k t _) => (lab_tag_matches l i k') || (label_tag_in_trace l i k t)
+    end.
+
+  Fixpoint label_in_trace (l : Lab) (k : Conf) (t : Tr k) : bool :=
+    match t with
+    | (Init s) => l ==b root
+    | (Step k' k t _) => (l ==b lab_of k') || (label_in_trace l k t)
+    end.
+
+  Lemma last_inst_self a l u t :
+     last_inst_of a (a, l, u) t = Some l.
+  Proof.
+    dependent induction t.
+    + simpl. destruct (root == root); firstorder. 
+    + simpl. destruct (a == a); firstorder. 
+  Qed.
+
+  Lemma last_inst_step l p i s k t step : 
+    l =/= p -> last_inst_of l k t = last_inst_of l (p, i, s) (Step (p, i, s) k t step).
+  Proof.
+    intros Hneq.
+    simpl. destruct (l == p); firstorder. 
+  Qed.
+    
+  Lemma last_inst_not_exists :
+    forall l k t, last_inst_of l k t = None <-> ~ exists i s, In k t (l, i, s).
+  Proof.
+    intros.
+    destruct k as [[p i] s].
+    dependent induction t.
+    + split; intros.
+      - simpl in H. destruct (l == root); try inversion H.
+        intro. destruct H0 as [j [r H0]].
+        inv_tr H0. contradiction c. reflexivity.
+      - simpl. destruct (l == root); try firstorder.
+        exfalso. rewrite e in *. eapply H. exists s. constructor.
+    + destruct k' as [[q j] r].
+      split; intros.
+      - simpl in H. destruct (l == p); [ inversion H |].
+        intro. eapply IHt; eauto.
+        destruct H0 as [m [w H0]]. exists m, w.
+        inv_tr H0; firstorder.
+      - simpl.
+        destruct (l == p).
+        * exfalso. apply H. rewrite e0. eauto using In.
+        * eapply IHt; eauto. intro. apply H.
+          destruct H0 as [m [w H0]].
+          eauto using In.
+  Qed.
+
+  Lemma last_inst_in :
+    forall l k t i, last_inst_of l k t = Some i -> exists s, In k t (l, i, s).
+  Proof.
+    intros. dependent induction t; simpl in H.
+    + destruct (l == root). 
+      - rewrite e in *. simpl in H. inversion H; subst. eexists. constructor.
+      - inversion H.
+    + destruct k as [[q j] r].
+      destruct (l == q).
+      - rewrite e0 in *. inversion H; subst. eexists. constructor.
+      - edestruct IHt; eauto. exists x. constructor. eassumption.
+  Qed.
+  
+  Lemma last_inst_in_inv :
+    forall k t l i s, In k t (l, i, s) -> exists j, last_inst_of l k t = Some j.
+  Proof.
+    intros. dependent induction t; simpl in H.
+    + destruct (l == root). 
+      - rewrite e in *. simpl. exists start_tag. destruct (root == root); firstorder.
+      - inv_tr H. firstorder.
+    + destruct k as [[q j] r].
+      destruct (l == q).
+      - rewrite e0 in *. simpl. exists j. destruct (q == q); firstorder.
+      - inv_tr H.
+        * firstorder.
+        * eapply IHt in H4. destruct H4 as [j' Hlast].
+          eexists. simpl. destruct (l == q).
+          ** contradiction c. 
+          ** eapply Hlast.
+  Qed.
+
+  Lemma precedes_same p m s w t :
+    Precedes (p, m, s) t (p, m, w) (p, m, s) -> w === s.
+  Proof.
+    intros H.
+    eapply precedes_implies_in_pred in H.
+    inv_tr H; try reflexivity. 
+    exfalso. eapply ivec_fresh; eauto.
+  Qed.
+
+  Lemma in_same_state p i s s' t :
+    In (p, i, s) t (p, i, s') -> s === s'.
+  Proof.
+    intros.
+    inv_tr H; try reflexivity.
+    + inv_tr H. reflexivity.
+      exfalso. eapply ivec_fresh; eauto.
+  Qed.
+
+    Lemma last_inst_step_pred p j r a l u t e : 
+    a =/= p -> last_inst_of a (p, j, r) (Step (p, j, r) (a, l, u) t e) = Some l.
+  Proof.
+    intros Hneq.
+    simpl.
+    destruct (a == p); firstorder. eapply last_inst_self.
+  Qed.
+
+  Lemma label_in_trace_in :
+    forall l k t, label_in_trace l k t = true <-> exists i s, In k t (l, i, s).
+  Proof.
+    intros.
+    induction t.
+    - simpl. split; intros.
+      + exists start_tag, s. conv_bool. rewrite H. constructor.
+      + destruct H as [i [s' Hin]].
+        inv_tr Hin.
+        unfold equiv_decb.
+        destruct (root == root); destruct (start_tag == start_tag); firstorder.
+    - destruct k as [[p j] s].
+      split; intros.
+      + destruct (l == p).
+        * rewrite e0 in *. exists j, s. constructor.
+        * destruct IHt as [IHt _].
+          simpl in H. conv_bool.
+          destruct H; [ exfalso; firstorder |].
+          destruct IHt as [r [s' Hin]]; eauto.
+          exists r, s'. eauto using In.
+      + destruct IHt as [_ IHt].
+        destruct H as [r [s' Hin]].
+        simpl.
+        inv_tr Hin; unfold equiv_decb.
+        * destruct (l == l); firstorder.
+        * destruct (l == p); simpl; auto; eapply IHt; eauto.
+  Qed.
+
+  Lemma not_label_in_trace_in :
+    forall l k t, label_in_trace l k t = false <-> ~ exists i s, In k t (l, i, s).
+  Proof.
+    intros.
+    split; intros. intro.
+    + rewrite <- negb_true_iff in H.
+      apply Is_true_eq_left in H.
+      apply negb_prop_elim in H.
+      apply H.
+      apply Is_true_eq_left.
+      apply label_in_trace_in; assumption.
+    + rewrite <- negb_true_iff.
+      apply Is_true_eq_true.
+      apply negb_prop_intro.
+      intro. apply H.
+      apply Is_true_eq_true in H0.
+      apply label_in_trace_in; assumption.
+  Qed.
+
+  Lemma label_tag_in_trace_in :
+    forall l i k t, label_tag_in_trace l i k t = true <-> exists s, In k t (l, i, s).
+  Proof.
+    intros.
+    induction t.
+    - simpl. split; intros.
+      + exists s. conv_bool. destruct H. rewrite H. rewrite H0. constructor.
+      + destruct H as [s' Hin].
+        inv_tr Hin.
+        unfold equiv_decb.
+        destruct (root == root); destruct (start_tag == start_tag); firstorder.
+    - destruct k as [[p j] s].
+      split; intros.
+      remember (lab_tag_matches l i (p, j, s)) as eq.
+      symmetry in Heqeq. simpl in Heqeq.
+      + destruct eq; conv_bool.
+        * destruct Heqeq. rewrite H0. rewrite H1. exists s. constructor.
+        * destruct IHt as [IHt _].
+          simpl in H. conv_bool.
+          destruct H; [ exfalso; firstorder |].
+          destruct IHt as [r Hin]; eauto.
+          exists r. eauto using In.
+      + destruct IHt as [_ IHt].
+        destruct H as [r Hin].
+        simpl.
+        inv_tr Hin; unfold equiv_decb.
+        * destruct (l == l); destruct (i == i); firstorder.
+        * destruct (l == p); destruct (i == j); simpl; auto; eapply IHt; eauto.
+  Qed.
+
+  Lemma not_label_tag_in_trace_in :
+    forall l i k t, label_tag_in_trace l i k t = false <-> ~ exists s, In k t (l, i, s).
+  Proof.
+    intros.
+    split; intros. intro.
+    + rewrite <- negb_true_iff in H.
+      apply Is_true_eq_left in H.
+      apply negb_prop_elim in H.
+      apply H.
+      apply Is_true_eq_left.
+      apply label_tag_in_trace_in; assumption.
+    + rewrite <- negb_true_iff.
+      apply Is_true_eq_true.
+      apply negb_prop_intro.
+      intro. apply H.
+      apply Is_true_eq_true in H0.
+      apply label_tag_in_trace_in; assumption.
+  Qed.
+
+  Definition lift (tr : Traces) : Hyper :=
+    fun ts => ts = tr.
+
+  Definition red_prod (h h' : Hyper) : Hyper :=
+    fun ts => h ts /\ h' ts.
+  
+End Evaluation.
