Unchanged.v
@@ -1,0 +1,263 @@
+
+Require Import Coq.Program.Utils.
+Require Import Lists.ListSet.
+Require Import List.
+
+Require Util Evaluation.
+
+Module Unchanged.
+  Import Evaluation.Evaluation Util.
+
+  Definition Unch := Lab -> Var -> set Lab.
+
+  Definition unch_concr (unch : Unch) : Traces :=
+    fun k => fun t => forall to i s u x, In k t (to, i, s) ->
+                              set_In u (unch to x) ->
+                              exists j r, Precedes k t (u, j, r) (to, i, s) /\
+                                     r x = s x.
+
+  (*
+  Definition unch_concr (unch : Unch) : Traces :=
+    fun k => fun t => forall to i s u x, In k t (to, i, s) ->
+                              set_In u (unch to x) ->
+                              exists d dj dr j r, is_def_lab x d /\
+                                             Precedes k t (d, dj, dr) (u, j, r) -> 
+                                             Precedes k t (u, j, r) (to, i, s) /\
+                                             r x = s x.
+  *)
+                           
+  Definition unch_join_ptw (d d' : set Lab) := set_inter Lab_dec' d d'. 
+
+  Definition unch_join (u u' : Unch) : Unch :=
+    fun l x => unch_join_ptw (u l x) (u' l x).
+
+  Definition unch_trans_local (unch : Unch) (q p : Lab) (x : Var) : set Lab :=
+    set_add Lab_dec' p (if is_def x q p then empty_set Lab else unch q x).
+
+  Definition unch_trans_ptw (unch : Unch) l x : set Lab :=
+    if Lab_dec' l root then set_add Lab_dec' root (empty_set Lab) else
+    let f := fun q acc => set_inter Lab_dec' q acc in
+    let t := fun q => unch_trans_local unch q l x in
+    fold_right f all_lab (map t (preds l)).
+      
+  Definition unch_trans (unch : Unch) : Unch :=
+    fun l x => unch_trans_ptw unch l x.
+
+  Lemma unch_trans_root : forall unch x, unch_trans unch root x = set_add Lab_dec' root (empty_set Lab).
+  Proof.
+    intros.
+    cut (preds root = nil); intros.
+    + unfold unch_trans, unch_trans_ptw.
+      destruct (Lab_dec' root root); firstorder.
+    + cut (forall q, ~ List.In q (preds root)); intros; eauto using list_emp_in, root_no_pred. 
+  Qed.
+
+  Inductive Front (u : Unch) : Var -> Lab -> Prop :=
+    | FrontDef : forall x p, is_def_lab x p -> Front u x p
+    | FrontIter : forall x l l' r r' p, l <> r ->
+                                   Front u x l ->
+                                   Front u x r ->
+                                   l' --> p ->
+                                   r' --> p ->
+                                   set_In l (u l' x) ->
+                                   set_In r (u r' x) ->
+                                   ~ set_In l (u r' x) ->
+                                   ~ set_In r (u l' x) ->
+                                   Front u x p.
+  
+  Lemma unch_trans_lem u to x unch :
+    set_In u (unch_trans unch to x) ->
+    u = to \/ (forall q, List.In q (preds to) -> (is_def x q to = false /\ set_In u (unch q x))).
+  Proof.
+    intros.
+    unfold unch_trans, unch_trans_ptw, unch_join_ptw, unch_trans_local in H.
+    induction (preds to); simpl in *.
+    - right. intros. inject H0.
+    - destruct (Lab_dec' to root).
+      + simpl in H. destruct H; [ subst | firstorder ]. eauto.
+      + eapply set_inter_elim in H.
+        destruct H as [Hin Hother].
+        eapply IHl in Hother. clear IHl.
+        inject Hother; [ eauto |].
+        destruct (Lab_dec' u to); subst; eauto.
+        right.
+        intros.
+        inject H0; [ subst | eauto].
+        destruct (is_def x q to).
+        * simpl in Hin. firstorder.
+        * eauto using set_add_elim2.
+  Qed. 
+
+  Lemma unch_correct :
+    forall unch k t,
+      sem_trace (unch_concr unch) k t -> unch_concr (unch_trans unch) k t.
+  Proof.
+    intros unch k t Hred.
+    unfold sem_trace in Hred.
+    destruct Hred as [k' [t' [step [Hconcr H]]]]; subst.
+    unfold unch_concr in *.
+    intros to i s u x.
+    intros Hin Hunch.
+    destruct (Lab_dec' to root); subst.
+    - unfold unch_trans, unch_trans_ptw in Hunch. destruct (Lab_dec' root root); [ | firstorder ].
+      simpl in Hunch. destruct Hunch; [ | firstorder ]. subst.
+      exists i, s. eauto using precedes_self.
+    - assert (Hpred := Hin).
+      eapply in_exists_pred in Hpred; try eassumption.
+      destruct Hpred as [q [j [r [Hpredin Hpred]]]].
+      assert (Hedge: q --> to) by (eauto using step_conf_implies_edge).
+      eapply unch_trans_lem in Hunch; try eassumption.
+      destruct (Lab_dec' to u) as [ | Hneq ]; subst.
+      + exists i, s. split; [ | reflexivity ].  eauto using precedes_self.
+      + destruct Hunch; [ firstorder |].
+        eapply H in Hedge. destruct Hedge as [Hndef Huin].
+        edestruct Hconcr as [j' [r' [Hprec Heq]]]; eauto.
+        exists j', r'. rewrite Heq. eauto using precedes_succ, no_def_untouched.
+  Qed.
+
+  (*
+  Lemma unch_dom (u : Unch) x l l' :
+    set_In l (u l' x) -> forall q, is_def_lab x q -> forall (π : Path q l'), PathIn l π.
+  Proof.
+  Admitted.
+
+  Lemma unch_path_exist (u : Unch) x l l' r :
+    set_In l (u l' x) -> ~ set_In r (u l' x) -> exists (π : Path l l'), ~ PathIn r π.
+  Proof.
+  Admitted.
+    
+  Lemma front_and_join (u : Unch) x p :
+    Front u x p <-> is_def_lab x p \/ exists d d' q q' (π : Path d q) (π' : Path d' q'), is_def_lab x d /\
+                                                                                 is_def_lab x d' /\
+                                                                                 q --> p /\ q' --> p /\
+                                                                                 DisjPaths π π'.
+  Proof.
+    split; intros.
+    - induction H; [ left; assumption | right ].
+      eapply unch_path_exist in H6; try eassumption.
+      eapply unch_path_exist in H7; try eassumption.
+      destruct H6 as [π Hπ], H7 as [π' Hπ'].
+      specialize (unch_dom _ _ _ _ H4). intro Hdom.
+      specialize (unch_dom _ _ _ _ H5). intro Hdom'.
+      assert (Hdom := unch_dom _ _ _ _).
+      assert (DisjPaths π π'). {
+        unfold DisjPaths.
+        intros q.
+        split; intros.
+        - 
+
+      destruct IHFront1, IHFront2.
+      + exists l, r, l', r', π, π'.
+        do 4 (split; [ assumption |]).
+        unfold DisjPaths.
+        admit.
+      + 
+
+      assert  
+      (*
+      destruct IHFront1, IHFront2.
+      + exists l, r, l', r'.
+        eexists. eexists. 
+        do 4 (split; [ assumption |]).
+        admit.
+      +
+       *)
+      admit.
+    - admit.
+                           
+  *)
+
+  (* Paths *)
+
+
+  (*
+  Section Disj.
+    Variable unch : Unch.
+    Variable s t f : Lab.
+    Variable x xs : Var.
+    Variable Hst : s --> t.
+    Variable Hsf : s --> f.
+    Variable Hbr : branch s = Some (t, f, x, xs).
+    Variable Hfp : unch_lfp unch.
+
+    Lemma unch_split_is_on_path dl to (p : Path f to) :
+      unch to xs = Some dl ->
+      PathIn dl p.
+    Proof.
+      intros Hunch.
+      induction p.
+      - rename p into f. simpl.
+        assertl (Hbrspec := branch_spec_var s t f x xs Hbr).
+        destruct Hbrspec as [Hl [Hr _]].
+        destruct (unch_trans_res unch s f xs Hsf).
+        + rewrite unch_lfp_trans_eq in H; try eassumption.
+          rewrite Hunch in H. inject H. reflexivity.
+        + destruct H as [_ [H _]].  rewrite H in *; firstorder.
+      - rename from into f. rename p into q. simpl.
+        destruct (unch_trans_res unch q to xs e).
+        + rewrite unch_lfp_trans_eq in H; try eassumption.
+          rewrite Hunch in H. inject H. left. reflexivity.
+        + destruct H as [_ [_ [_ H]]].
+          rewrite unch_lfp_trans_eq in H; try eassumption.
+          rewrite H in Hunch. right. eauto.
+    Qed.
+    
+    Lemma unch_split_exists {to} (p : Path f to) :
+      exists dl, unch to xs = Some dl /\ PathIn dl p.
+    Proof.
+      induction p.
+      - rename p into f. simpl.
+        assert (Hbrspec := branch_spec_var s t f x xs Hbr).
+        destruct Hbrspec as [Hl [Hr _]].
+        destruct (unch_trans_res unch s f xs Hsf).
+        + rewrite unch_lfp_trans_eq in H; try eassumption.
+          exists f. split; [ eauto | reflexivity ].
+        + destruct H as [_ [H _]]. rewrite H in *; firstorder.
+      - rename from into f. rename p into q. simpl.
+        destruct (unch_trans_res unch q to xs e).
+        + rewrite unch_lfp_trans_eq in H; try eassumption.
+          exists to. split; eauto. 
+        + destruct H as [_ [_ [_ H]]].
+          rewrite unch_lfp_trans_eq in H; try eassumption.
+          destruct IHp as [dl [IHp Hin]]; try eassumption. rewrite IHp in H.
+          exists dl. eauto. 
+    Qed.
+
+    Variable l r : Lab.
+
+    Section PathsGiven.
+      Variable a : Path t l.
+      Variable b : Path f r.
+  
+      Lemma unch_disj_l :
+        disjoint a b ->
+        exists dl dr, unch l xs = Some dl /\ unch r xs = Some dr /\ dl =/= dr.
+      Proof.
+        intros Hdis.
+        unfold disjoint in Hdis.
+        destruct Hdis as [Hl Hr].
+        induction a as [t | t].
+        - destruct (branch_spec_var s t f x xs Hbr) as [Hdef _].
+          destruct (unch_trans_res unch s t xs Hst); rewrite unch_lfp_trans_eq in H; try eassumption.
+          + destruct (unch_split_exists b) as [dr [Hu Hp]].
+            exists t, dr. repeat split; try eassumption.
+            intro. eapply Hl. constructor. rewrite H0. assumption.
+          + destruct H as [_ [H _]]. rewrite Hdef in H. firstorder.
+        - rename p0 into b', p into l.
+          destruct IHp; try eassumption.
+          + intros. apply Hl. simpl. auto.
+          + intros. apply Hr in H. contradict H. simpl. auto.
+          + destruct H as [dr [Hul [Hur Hneq]]].
+            destruct (unch_trans_res unch l to xs e); rewrite unch_lfp_trans_eq in H; try eassumption.
+            * exists to, dr. repeat split; eauto. 
+              intro. eapply (Hl to). simpl. left. reflexivity. eapply unch_split_is_on_path. auto.
+              rewrite H0. eassumption.
+            * destruct H as [_ [_ [_ H]]].
+              rewrite H. eauto.
+      Qed.
+
+*)
+
+
+
+End Unchanged.
