Uniana.v
@@ -1,0 +1,160 @@
+Require Import Coq.Classes.EquivDec.
+Require Import Coq.Classes.RelationClasses.
+Require Import Coq.Bool.Bool.
+Require Import Coq.Logic.Eqdep.
+Require Import Coq.Logic.Eqdep_dec.
+Require Import Coq.Logic.Decidable.
+Require Import Coq.Program.Equality.
+Require Import Coq.Program.Utils.
+Require Import Lists.ListSet.
+Require Import List.
+Require Import Nat. 
+
+Require Util Graph Evaluation Unchanged Disjoint UniquePI.
+
+Module Uniana.
+  Import Util Evaluation.Evaluation Disjoint.Disjoint Unchanged.Unchanged UniquePI.UniquePI.
+  
+  Parameter init_uni : Var -> Prop.
+
+  Definition UniState := Var -> bool.
+         
+  Parameter abs_uni_eff : UniState -> UniState.
+
+  Definition uni_state_concr (uni : UniState) : State -> State -> Prop :=
+    fun s => fun s' => forall x, uni x = true -> s x = s' x.
+
+  Parameter local_uni_corr : forall uni p i q j s s' qs qs', 
+      uni_state_concr uni s s' ->
+      eff (p, i, s) = Some (q, j, qs) ->
+      eff (p, i, s') = Some (q, j, qs') ->
+      uni_state_concr (abs_uni_eff uni) qs qs'.
+
+  Definition uni_concr (u : Uni) : Hyper :=
+    fun ts => forall t t' tr tr', ts t tr -> ts t' tr' ->
+                          forall x p i s s', In t tr ((p, i), s) ->
+                                        In t' tr' ((p, i), s') ->
+                                        u p x = true -> s x = s' x.
+  
+  Definition uni_trans (uni : Uni) (upi : Upi) (unch : Unch) : Uni :=
+    fun p => if p == root then uni root
+             else fun x => ((join_andb (map (fun spl => 
+                                           match spl with (s, x) => uni s x &&
+                                                upi_trans upi uni s p end) (splits p))) 
+                              && (join_andb (map (fun q => abs_uni_eff (uni q) x) (preds p)))
+                              && (join_andb (map (fun q => upi_trans upi uni q p) (preds p)))
+                           )
+                        || join_orb (map (fun q => (q <>b p) && uni q x && upi_trans upi uni q p) (unch_trans unch p x)).
+
+  Lemma uni_trans_root_inv :
+    forall uni hom unch x, uni_trans uni hom unch root x = uni root x.
+  Proof.
+    intros.
+    unfold uni_trans.
+    destruct (equiv_dec root root).
+    reflexivity.
+    exfalso. apply c. reflexivity.
+  Qed.
+
+  Lemma uni_correct :
+    forall uni upi unch t,
+        sem_hyper (red_prod (red_prod (uni_concr uni) (upi_concr upi)) (lift (unch_concr unch))) t ->
+        uni_concr (uni_trans uni upi unch) t.
+  Proof.
+    intros uni upi unch t Hred.
+    unfold sem_hyper in Hred.
+    destruct Hred as [ts [Hconcr Hstep]].
+    intros k k' tr tr' Hsem Hsem' x p i s s'.
+    intros HIn HIn' Htrans.
+
+    assert (upi_concr (upi_trans upi uni) t) as HCupi. {
+      apply upi_correct. 
+      destruct Hconcr as [[_ Hhom] _].
+      exists ts; auto.
+    }
+
+    assert (unch_concr (unch_trans unch) k tr) as HCunch. {
+      destruct Hconcr as [[_ _] Hunch].
+      unfold lift in *; subst.
+      apply unch_correct. assumption.
+    } 
+    
+    assert (unch_concr (unch_trans unch) k' tr') as HCunch'. {
+      destruct Hconcr as [[_ _] Hunch].
+      unfold lift in *; subst.
+      apply unch_correct. assumption.
+    }
+
+    destruct Hconcr as [[HCuni HCupi'] _].
+
+    subst.
+    unfold uni_trans in Htrans. 
+    assert (X := Hsem). destruct X as [l [ltr [lstep [Hts Hlstep]]]]; subst.
+    assert (X := Hsem'). destruct X as [l' [ltr' [lstep' [Hts' Hlstep']]]]; subst.
+
+    destruct (p == root); [ subst | ].
+    + rewrite e in *; clear e.
+      inv_tr HIn.
+      - exfalso. eauto using start_no_tgt. 
+      - inv_tr HIn'; [ exfalso |]; eauto using start_no_tgt. 
+
+    + conv_bool.
+      destruct Htrans as [Htrans | Hunch].
+        (* The uni/hom case *)
+      - destruct Htrans as [[Hsplit Hpred] Hupi].
+        eapply in_pred_exists in HIn; try eassumption.
+        eapply in_pred_exists in HIn'; try eassumption.
+        destruct HIn as [q [j [r [HIn Hstep]]]].
+        destruct HIn' as [q' [j' [r' [HIn' Hstep']]]].
+        assert (List.In q (preds p)) as Hqpred by (eauto using step_conf_implies_edge).
+
+        cut (q' = q); intros; subst.
+        * cut (j' = j); intros; subst.
+          -- eapply (local_uni_corr (uni q) q j p i r r' s s'); try eassumption.
+             ** unfold uni_state_concr. intros.
+                unfold uni_concr in HCuni .
+                eapply (HCuni l l' ltr ltr' Hts Hts' x0 q j); eassumption.
+             ** eapply join_andb_true_iff in Hpred; try eassumption.
+          -- (* unique preceding instances *)
+             eapply join_andb_true_iff in Hupi; try eassumption.
+             assert (p =/= q) by (symmetry; eauto using step_conf_implies_edge, no_self_loops).
+             eapply HCupi; [ eapply Hsem | eapply Hsem' | eassumption | | ].
+             all: eauto using precedes_step.
+        * (* disjoint paths! *)
+          destruct (q == q') as [ Heq | Hneq ]; [ eauto | exfalso ].
+          assert (List.In q' (preds p)) as Hqpred' by (eauto using step_conf_implies_edge).
+          unfold upi_concr in HCupi.
+          eapply (join_andb_true_iff _ _ Hupi) in Hqpred'.
+          eapply (join_andb_true_iff _ _ Hupi) in Hqpred.
+          symmetry in Hneq.
+          eapply disjoint with (q := q) (step := lstep) in Hneq; eauto.
+          ++ destruct Hneq as [br [y [yb [Hwit Hspl]]]].
+             destruct Hwit as [m [u' [u [Hney [Hinbr' [Hinbr _]]]]]].
+             eapply join_andb_true_iff in Hsplit; try eapply Hspl. simpl in Hsplit. conv_bool.
+             destruct Hsplit as [Hsplit _].
+             apply Hney.
+             cut (u' y = u y); intros. rewrite H. reflexivity.
+             eapply HCuni; [ exact Hts' | exact Hts | | | ]; eauto.
+          ++ intros.
+             eapply HCupi; eauto.
+             eapply (join_andb_true_iff _ _ Hsplit) in H.
+             conv_bool. destruct H as [_ H]. eassumption.
+        (* The unch case *)
+      - rename Hunch into H.
+        eapply join_orb_true_iff in H.
+        destruct H as [u H].
+        conv_bool.
+        destruct H as [Hunch [[Hneq' Huni] Hupi]].
+        specialize (HCunch p i s u x HIn Hunch).
+        specialize (HCunch' p i s' u x HIn' Hunch).
+        destruct HCunch as [j [r [Hprec Heq]]]; try eassumption.
+        destruct HCunch' as [j' [r' [Hprec' Heq']]]; try eassumption.
+        rewrite <- Heq. rewrite <- Heq'.
+        cut (j' = j); intros.
+        * subst j'. eauto using precedes_step_inv.  
+        * eapply (HCupi _ _ _ _ Hsem Hsem'); eauto. 
+  Qed.
+
+
+End Uniana.
+      
