UniquePI.v
@@ -1,0 +1,194 @@
+Require Import Coq.Classes.EquivDec.
+Require Import Coq.Classes.RelationClasses.
+Require Import Coq.Bool.Bool.
+Require Import Coq.Logic.Eqdep.
+Require Import Coq.Logic.Eqdep_dec.
+Require Import Coq.Logic.Decidable.
+Require Import Coq.Program.Equality.
+Require Import Coq.Program.Utils.
+Require Import Lists.ListSet.
+Require Import List.
+Require Import Nat.
+
+Require Evaluation Disjoint Util.
+
+Module UniquePI.
+  Export Evaluation.Evaluation Disjoint.Disjoint Util.
+  
+  Definition Upi := Lab -> Lab -> bool.
+
+  Definition Uni := Lab -> Var -> bool.
+
+  Definition upi_prop q p k k' t t' :=
+    forall j j' i r r' s s', Precedes k t (q, j, r) (p, i, s) ->
+                             Precedes k' t' (q, j', r') (p, i, s') ->
+                             j' = j.
+
+  Definition upi_concr (upi : Upi) : Hyper :=
+    fun ts => forall k k' t t',
+        ts k t -> ts k' t' ->
+        forall q p, upi q p = true -> upi_prop q p k k' t t'.
+
+  Parameter lh_p_le_q : Lab -> Lab -> list (Lab * Var).
+  
+  Parameter lh_p_le_q_spec :
+    forall (p q le : Lab) (x : Var), List.In (le,x) (lh_p_le_q p q)
+                               <-> (exists (lh : Lab),
+                                     le --> lh
+                                     /\ AcyPath lh p
+                                     /\ AcyPath p le
+                                     /\ AcyPath le q
+                                     /\ exists a b, branch le = Some (a, b, x)).
+
+  Parameter loop_splits : Lab -> Lab -> list (Lab * Var).
+
+  Parameter loop_splits_spec :
+    forall (p q s : Lab) (x : Var), List.In (s,x) (loop_splits p q)
+                               <-> (exists (lh le le' : Lab),
+                                     le --> lh
+                                     /\ AcyPath lh p
+                                     /\ AcyPath p le
+                                     /\ AcyPath lh le'
+                                     /\ AcyPath le q
+                                     /\ le =/= le'
+                                     /\ List.In (s,x) (splits le')).
+   
+  Definition upi_trans (upi : Upi) (uni : Uni) : Upi :=
+    fun p
+    => fun q
+      => join_andb (map (fun spl
+                    => match spl with (s,x) => uni s x end)
+                           (lh_p_le_q p q
+                           ++  loop_splits p q))
+                  && (join_andb (map (upi p) (preds q))).
+
+    Lemma last_inst_upi_prop {p br m m' w w' q q' i j j' s s' r r' step step' t t'} :
+    let tr := (Step (p, i, s) (q, j, r) t step) in
+    let tr' := (Step (p, i, s') (q', j', r') t' step') in
+    upi_prop br p (p, i, s) (p, i, s') tr tr' ->
+    In (q, j, r) t (br, m, w) ->
+    In (q', j', r') t' (br, m', w') ->
+    p =/= br ->
+    last_inst_of br (q, j, r) t = last_inst_of br (q', j', r') t'.
+  Proof.
+    simpl. intros Hupi Hin Hin' Hneq.
+    eapply last_inst_in_inv in Hin.
+    eapply last_inst_in_inv in Hin'.
+    destruct Hin as [k Hlast].
+    destruct Hin' as [k' Hlast'].
+    rewrite Hlast. rewrite Hlast'.
+    unfold upi_prop in Hupi.
+    eapply last_inst_precedes in Hlast. destruct Hlast as [u Hprec]. 
+    eapply last_inst_precedes in Hlast'. destruct Hlast' as [u' Hprec']. 
+    symmetry. f_equal. eauto using Precedes.
+  Qed.
+  
+  Lemma upi_comm q p k k' t t' :
+    upi_prop q p k k' t t' ->
+    upi_prop q p k' k t' t.
+  Proof.
+    unfold upi_prop in *. intros. symmetry. eauto.
+  Qed.
+  
+  Lemma upi_correct :
+    forall upi uni t, sem_hyper (upi_concr upi) t -> upi_concr (upi_trans upi uni) t.
+  Proof.
+    intros.
+    unfold sem_hyper in H. destruct H as [ts [Hconcr Htrace]].
+    unfold upi_concr. intros.
+    unfold upi_prop. intros.
+    induction H2; induction H3.
+    Focus 1. Unfocus. Focus 2.
+    apply IHPrecedes. 
+    Unfocus. Focus 3. Unfocus. Focus 5. Unfocus. Focus 6. Unfocus. Focus 9.
+  Admitted.
+
+  Lemma upi_prefix {b p i s s' q j r q' j' r' k k' kp kp' pstep pstep' t t' tr tr'}
+        (step : eff (q, j, r) = Some (p, i, s)) 
+        (step' : eff (q', j', r') = Some (p, i, s')) :
+    Prefix (q, j, r) tr kp t ->
+    Prefix (q', j', r') tr' kp' t' ->
+    upi_prop b p k k' (Step k kp t pstep) (Step k' kp' t' pstep') ->
+    upi_prop b p (p, i, s) (p, i, s') (Step (p, i, s) (q, j, r) tr step)
+             (Step (p, i, s') (q', j', r') tr' step').
+  Proof.
+    intros Hupi Hprefix Hprefix'.
+    repeat split; try assumption; unfold upi_prop in *; intros; eauto using precedes_prefix_inv.
+  Qed.
+
+
+  Lemma disjoint p q q' i j j' s s' r r' l l' k k' tr tr' step step'
+        (Hstep : eff (q, j, r) = Some (p, i, s))
+        (Hstep' : eff (q', j', r') = Some (p, i, s')) :
+    let ltr := (Step l k tr step) in
+    let ltr' := (Step l' k' tr' step') in 
+    In k tr (q, j, r) ->
+    In k' tr' (q', j', r') ->
+    upi_prop q p l l' ltr ltr' ->
+    upi_prop q' p l l' ltr ltr' ->
+    (forall spl x, List.In (spl, x) (splits p) -> upi_prop spl p l l' ltr ltr') ->
+    q' =/= q ->
+    exists br x xb, DivergenceWitness br x xb k' k tr' tr /\
+               List.In (br, x) (splits p).
+  Proof.
+    simpl.
+    intros Hpref Hpref' Hupi Hupi' Hspl Hneq.
+    eapply in_prefix in Hpref.
+    eapply in_prefix in Hpref'.
+    destruct Hpref as [t [Hpref Hqin]].
+    destruct Hpref' as [t' [Hpref' Hqin']].
+    eapply (upi_prefix Hstep Hstep') in Hupi; try eassumption.
+    eapply upi_comm in Hupi'.
+    eapply (upi_prefix Hstep' Hstep) in Hupi'; try eassumption.
+    eapply upi_comm in Hupi'.
+
+    cut (exists br x xb, DivergenceWitness br x xb (q', j', r') (q, j, r) t' t /\
+                    List.In (br, x) (splits p)); intros.
+    destruct H as [br [x [xb [Hwit Hinbr]]]].
+    unfold DivergenceWitness in *.
+    destruct Hwit as [m [u [u' [Hneqv [Hin [Hin' Hbr]]]]]].
+    exists br, x, xb. split; [|eassumption].
+    exists m, u, u'. repeat split; eauto using in_prefix_in.
+
+    destruct (label_tag_in_trace q j (q', j', r') t') eqn:Hin,
+             (label_tag_in_trace q' j' (q, j, r) t) eqn:Hin';
+      eauto using disjoint_contains.
+    + symmetry in Hneq. edestruct disjoint_contains as [br [x [xb Hcont]]]; eauto. 
+      exists br, x, xb. rewrite witness_commutative. eauto.
+    + edestruct not_contains_label_tag_last_common; eauto.
+      - destruct H as [br [x [xb [Hdis [Hinbr Hwit]]]]].
+        destruct Hinbr as [m' [w' Hinbr]].
+        clear Hupi Hupi'. exists br, x, xb.
+        destruct Hdis as [m [w [Hinbr' [Pbrq [Hbr Hdis]]]]]. 
+        assert (List.In (br, x) (splits p)). {
+          eapply (splits_spec).
+          exists q', q. eexists. exists Pbrq.
+          repeat split; eauto using step_conf_implies_edge. 
+        }
+        specialize (Hspl _ _ H).
+        split; [ | assumption].
+        eapply (upi_prefix Hstep Hstep' Hpref Hpref') in Hspl.
+        eapply Hwit. symmetry. eapply last_inst_upi_prop; try eassumption.
+        destruct (p == br); try eassumption.
+        rewrite <- e in *. clear e. exfalso. eapply Hneq.
+        eapply in_out_spec; eauto using step_conf_implies_edge.
+      - clear Hspl.
+        assert (p =/= q /\ p =/= q'). {
+          split; symmetry; eauto using step_conf_implies_edge, no_self_loops.
+        }
+        destruct H0 as [Hnqp Hnqp'].
+        exfalso.
+        destruct H as [[j'' [Hneq'' Hin'']] | [j'' [Hneq'' Hin'']]].
+        * eapply last_inst_precedes in Hin''.
+          destruct Hin'' as [s'' Hin''].
+          eapply Hneq''. symmetry. eapply Hupi.
+          ++ repeat constructor. eassumption.
+          ++ eauto using Precedes.
+        * eapply last_inst_precedes in Hin''.
+          destruct Hin'' as [s'' Hin''].
+          eapply Hneq''. eapply Hupi'.
+          ++ eauto using Precedes.
+          ++ repeat constructor. eassumption.
+  Qed.
+  
+End UniquePI.
